LeanMqtt/Packets/Proofs.lean
@@ -50,4 +50,17 @@ theorem Packet.reconstruct {p : Packet} {input rest : List UInt8} :
   intro h
   exact PredType.reconstruct _ h
 
+theorem RawPacket.serialize_len (p : RawPacket) :
+    p.serialize.length = GetByteSize.byteSize p := by
+  simp only [RawPacket.serialize, GetByteSize.byteSize, RawPacket.byteSize]
+  simp only [List.length_append]
+  simp only [FixedHeader.serialize_len p.fh,
+    VarHeader.serialize_len p.vh,
+    Payload.serialize_len p.pl]
+  rfl
+
+theorem Packet.serialize_len (p : Packet) :
+    p.serialize.length = GetByteSize.byteSize p := by
+  exact PredType.serialize_len p RawPacket.serialize_len
+
 end Mqtt
